begin axiomitizing APL.

src/Logic/APL.v
@@ -3,6 +3,10 @@ Require Import Coq.Classes.RelationClasses.
 Require Import Coq.Classes.Morphisms.
 Require Import stdpp.base.
 
+From iris.proofmode Require Import base .
+
+From MyProject.src.Logic Require Import SysF typing.
+
 Reserved Notation "'emp'".
 Reserved Notation "(⊢)" (at level 99).
 Reserved Notation "P ⊢ Q" (at level 99, Q at level 200, right associativity).
@@ -11,6 +15,7 @@ Reserved Notation "P ∨ Q" (at level 85, right associativity, format "P '/' ∨
 Reserved Notation "P → Q"
 (at level 99, Q at level 200, right associativity,
  format "'[' P '/' → '/' '[' Q ']' ']'").
+ 
 
 
 
@@ -19,13 +24,28 @@ Module APL.
     Universe Logic.
     Universe Quant.
 
+    Import SysF.
+    Import typing.
+
+    Definition ty (t : type) : Type := sig (fun (e : expr) => typed [] e t).
+
+    Definition Rel (t1 t2 : type) {P : Type} : Type := ty t1 -> ty t2 -> P.
+    Definition Rel' {P : Type} : Type := @sigT (prod type type)(fun p => @Rel p.1 p.2 P).
+
+    Definition Raw_Rel {PROP : Type} : Type := (expr * expr) -> PROP.
+
     Section laws.
         Context {PROP : Type}.
     
         Context {apl_entails : PROP -> PROP -> Prop}.
         Context {apl_and : PROP -> PROP -> PROP}.
+        Context {apl_emp : PROP}.
         Context {apl_imp: PROP -> PROP -> PROP}.
         Context {apl_forall : forall A, (A -> PROP) -> PROP}.
+        Context {apl_forall_term : forall (t : type), (ty t -> PROP) -> PROP}.
+        Context {apl_forall_type : (type -> PROP) -> PROP}.
+        Context {apl_rel_sub : type -> list (@Rel' PROP) -> @Rel' PROP}.
+        Context {apl_rel_sub' : type -> list (@Raw_Rel PROP) -> @Raw_Rel PROP}.
 
         Bind Scope apl_scope with PROP.
 
@@ -33,6 +53,17 @@ Module APL.
         Local Infix "⊢" := apl_entails.
         Local Infix "∧" := apl_and : apl_scope.
         Local Infix "→" := apl_imp : apl_scope.
+
+        Definition apl_iff (P Q : PROP) : PROP := 
+            apl_and (apl_imp P Q) (apl_imp Q P).
+
+        Definition apl_rel_iff {t1 t2 : type} (R1 R2 : @Rel t1 t2 PROP) : PROP := 
+        apl_forall_term t1 (fun tm1 => 
+        apl_forall_term t2 (fun tm2 => 
+            apl_iff (R1 tm1 tm2) (R2 tm1 tm2))).
+
+        Definition Rel_to_Rel' (t1 t2 : type) (R : @Rel t1 t2 PROP) : @Rel' PROP := 
+            existT (pair t1 t2) R.
 
         Record AplLaws := {
             apl_entails_po : PreOrder apl_entails ;
@@ -44,25 +75,54 @@ Module APL.
             apl_impl_intro_r P Q R : (P ∧ Q ⊢ R) -> P ⊢ Q → R;
             apl_impl_elim_l' P Q R : (P ⊢ Q → R) -> P ∧ Q ⊢ R;
 
-            apl_forall_term_intro {A} P (Ψ : A -> PROP) : 
+            apl_forall_intro {A} P (Ψ : A -> PROP) : 
                 (forall a, P ⊢ Ψ a) -> P ⊢ apl_forall _ (fun a => Ψ a );
+
+            apl_forall_elim {A} {Ψ : A -> PROP} a : apl_forall _ (fun a => Ψ a ) ⊢ Ψ a;
+
+            apl_forall_term_intro {t} P (Ψ : ty t -> PROP) : 
+                (forall tm, P ⊢ Ψ tm) -> P ⊢ apl_forall_term _ (fun tm => Ψ tm );
+
+            apl_forall_term_elim {t} {Ψ : ty t -> PROP} a : apl_forall_term _ (fun a => Ψ a ) ⊢ Ψ a;
+
+            apl_forall_type_intro P (Ψ : type -> PROP) : 
+                (forall t, P ⊢ Ψ t) -> P ⊢ apl_forall_type (fun t => Ψ t );
+
+            apl_forall_type_elim  {Ψ : type -> PROP} t : apl_forall_type (fun t => Ψ t ) ⊢ Ψ t;
+
+            (* relational substitution laws *)
+            apl_rel_sub_arrow (rho : list (@Rel' PROP)) (t1 t2 : type) : 
+                apl_emp ⊢ (@apl_rel_iff t1 t2 
+                    (apl_rel_sub (TArrow t1 t2) rho) 
+                    (apl_rel_sub (TArrow t1 t2) rho)) ;
+
         }.
     End laws.
+    Check sig.
+    Print prod.
+
+
+
 
     Structure apl := APL {
         apl_car :> Type@{Logic};
         apl_entails : apl_car -> apl_car -> Prop;
         apl_emp : apl_car;
+        (* 
+            this gets mapped to "interp"?, 
+            the definition of the binary logical relation on exrpessions
+         *)
+        apl_rel_sub : type -> list (@Rel' apl_car) -> @Rel' apl_car;
         (* equality *)
         (* relations *)
         apl_imp : apl_car -> apl_car -> apl_car ;
         apl_forall :  forall A : Type@{Quant}, (A -> apl_car) -> apl_car;
-(*         (* forall term *)
-        apl_forall_term : forall A : Type@{Quant}, (A -> apl_car) -> apl_car;
+        (* forall term *)
+        apl_forall_term : forall (t : type), (ty t -> apl_car) -> apl_car;
         (* forall type *)
-        apl_forall_type : forall A : Type@{Quant}, (A -> apl_car) -> apl_car;
+        apl_forall_type : (type -> apl_car) -> apl_car;
         (* forall rel *)
-        apl_forall_rel : forall A : Type@{Quant}, (A -> apl_car) -> apl_car; *)
+        apl_forall_rel : forall {t1} {t2}, ((@Rel t1 t2 apl_car) -> apl_car) -> apl_car; 
         apl_and : apl_car -> apl_car -> apl_car;
         apl_or : apl_car -> apl_car -> apl_car;
         apl_exist : forall A : Type@{Quant}, (A -> apl_car) -> apl_car;
@@ -72,7 +132,7 @@ Module APL.
         apl_exist_type : forall A : Type@{Quant}, (A -> apl_car) -> apl_car;
         (* exists rel *)
         apl_exist_rel : forall A : Type@{Quant}, (A -> apl_car) -> apl_car; *)
-        apl_laws : @AplLaws apl_car apl_entails apl_and apl_imp apl_forall
+        apl_laws : @AplLaws apl_car apl_entails apl_and apl_imp apl_forall apl_forall_term apl_forall_type
     }.
 
     Declare Scope apl_scope.
@@ -102,11 +162,17 @@ Module APL.
     Infix "∨" := apl_or : apl_scope.
     Notation "(∨)" := apl_or (only parsing) : apl_scope.
     Infix "→" := apl_imp : apl_scope.
-(* 
+
     Notation "∀ x .. y , P" :=
-    (apl_forall (λ x, .. (apl_forall (λ y, P%I)) ..)) : apl_scope.
+    (apl_forall (λ x, .. (apl_forall (λ y, P%A)) ..)) : apl_scope.
     Notation "∃ x .. y , P" :=
-    (apl_exist (λ x, .. (apl_exist (λ y, P%I)) ..)) : apl_scope. *)
+    (apl_exist (λ x, .. (apl_exist (λ y, P%A)) ..)) : apl_scope. 
+
+Check apl_forall_type _.
+    Notation "∀ty x , P" :=
+    (apl_forall_type _ (λ x, P%A))  (at level 100) : apl_scope.
+
+
     Notation "(⊢)" := apl_entails (only parsing) : stdpp_scope.
     Notation "P ⊢ Q" := (apl_entails P%A Q%A) : stdpp_scope.
 
@@ -143,17 +209,32 @@ Definition imp (A B : Prop) := forall (_ : A ), B.
 
 Check @AplLaws Prop imp and imp all.
 
-Lemma instance : @AplLaws Prop imp and imp all.
+(* Lemma instance : @AplLaws Prop imp and imp all.
 Proof.
     constructor; unfold imp in *.
     (* These laws already exist in Logic module *)
     2:{ intros P Q [P' Q']. exact P'.  }
     6:{ intros. unfold all. intros. pose proof (H x H0). exact H1. }
 Admitted.
+ *)
+ Import typing.
+
+Definition all_term : forall (t : type), (ty t -> Prop) -> Prop := 
+fun t P => (forall e, P e).
+
+Lemma instance : apl.
+    apply (APL Prop imp True imp all all_term (@all type) and or ex).
+    constructor.
+    10:{
+        intros. unfold imp. intros. unfold all_term in H. exact (H a).
+    }
+    9:{
+        intros. unfold imp. intros. unfold all_term. intros. exact (H e H0).
+    }
+Abort.
 
 Section huh.
     Context {PROP : apl}.
-    Context {term : Type}.
     Check @apl_imp PROP.
     Check apl_imp.
     Notation "P ⊢ Q" := (@apl_entails PROP P%A Q%A) : stdpp_scope.
@@ -164,16 +245,121 @@ Section huh.
 
 Fail Lemma  thing (P Q : PROP) : ⊢ ((Q → True) ∧ Q)%A.
 
-Lemma thing P Q  : P ∧ (P → Q)⊢ Q.
+Lemma thing P Q  : P ∧ (P → Q) ⊢ Q.
 Proof.
     Check apl_and_intro (apl_laws PROP).
     Check apl_impl_elim_l' (apl_laws PROP).
     apply (apl_impl_elim_l' (apl_laws PROP)).
 Abort.
 
-Lemma foo P : ⊢ @apl_forall PROP term (fun x => P).
+(* Lemma foo P : ⊢ @apl_forall PROP term (fun x => P).
 Proof.
-    apply (apl_forall_term_intro (apl_laws PROP)).
+    apply (apl_forall_intro (apl_laws PROP)).
     intros.
-    Check apl_forall_term_intro (apl_laws PROP).
+    Check apl_forall_intro (apl_laws PROP).
 Check @apl_forall PROP term.
+Abort. *)
+
+Lemma foo P : ⊢ @apl_forall_type PROP (fun x => P x).
+Proof.
+    apply (apl_forall_type_intro (apl_laws PROP)).
+    intros.
+(*     eapply (apl_forall_type_elim (apl_laws PROP)).
+    intros *)
+Abort.
+End huh.
+Section tactics.
+    Context {PROP  : apl}.
+
+    Inductive env : Type :=
+    | Enil : env 
+    | Esnoc : env  → ident → PROP → env .
+
+    Fixpoint env_lookup (i : ident) (Γ : env ) : option PROP :=
+    match Γ with
+    | Enil => None
+    | Esnoc Γ j x => if ident_beq i j then Some x else env_lookup i Γ
+    end.
+
+    Notation "Γ !! j" := (env_lookup j Γ).
+
+    Fixpoint env_delete  (i : ident) (Γ : env) : env :=
+    match Γ with
+    | Enil => Enil
+    | Esnoc Γ j x => if ident_beq i j then Γ else Esnoc (env_delete i Γ) j x
+    end.
+
+
+    Inductive env_wf  : env → Prop :=
+    | Enil_wf : env_wf Enil
+    | Esnoc_wf Γ i x : Γ !! i = None → env_wf Γ → env_wf (Esnoc Γ i x).
+
+
+(*     Global Arguments Enil {_}.
+    Global Arguments Esnoc {_} _ _ _.
+    Global Instance: Params (@Enil) 1 := {}.
+    Global Instance: Params (@Esnoc) 1 := {}. *)
+
+    Definition of_envs' {PROP : apl} (Γ : env) : PROP := emp.
+   (*  (⌜envs_wf' Γp Γs⌝ ∧ env_and_persistently Γp )%A. *)
+
+  Global Instance: Params (@of_envs') 1 := {}.
+  Definition of_envs {PROP : apl} (Δ : env ) : PROP :=
+    of_envs' Δ .
+  Global Instance: Params (@of_envs) 1 := {}.
+  Global Arguments of_envs : simpl never.
+  
+  Local Definition pre_envs_entails_def {PROP : apl} (Γ : env) (Q : PROP) :=
+    of_envs' Γ ⊢ Q.
+  Local Definition pre_envs_entails_aux : seal (@pre_envs_entails_def).
+  Proof. by eexists. Qed.
+  Local Definition pre_envs_entails := pre_envs_entails_aux.(unseal).
+  Local Definition pre_envs_entails_unseal :
+  @pre_envs_entails = @pre_envs_entails_def := pre_envs_entails_aux.(seal_eq).
+
+    Definition envs_entails {PROP : apl} (Δ : env) (Q : PROP) : Prop :=
+  pre_envs_entails PROP Δ  Q.
+
+Definition envs_entails_unseal :
+  @envs_entails = λ PROP (Δ : env ) Q, (of_envs Δ ⊢ Q).
+  Proof. unfold envs_entails. Admitted.
+
+
+
+Global Arguments envs_entails {PROP} Δ Q%_A.
+Global Instance: Params (@envs_entails) 1 := {}.
+
+Lemma tac_start {P : PROP} : envs_entails (Enil) P → ⊢ P.
+Proof.
+  rewrite envs_entails_unseal. unfold of_envs. unfold of_envs'. intros. done.
+Qed.
+
+Lemma tac_pure  Δ i P (φ : Prop) (Q : PROP) :
+  env_lookup i Δ = Some P →
+
+  (φ → envs_entails (env_delete i  Δ) Q) → envs_entails Δ Q.
+Proof. 
+    intros.
+    rewrite envs_entails_unseal.
+    rewrite envs_entails_unseal in H0.
+Admitted.
+
+End tactics.
+
+Section test.
+    Context {PROP : apl}.
+    Lemma thing (P Q : PROP)  : ⊢ ((P ∧ (P → Q)) → Q).
+    Proof.
+        apply (apl_impl_intro_r (apl_laws PROP)).
+        pose proof ()
+        apply tac_start.
+
+        eapply tac_pure.
+
+        rewrite envs_entails_unseal.
+        unfold of_envs.
+        unfold of_envs'.
+
+
+
+End huh.
