src/Logic/typing.v
@@ -1,0 +1,91 @@
+From MyProject.src.Logic Require Export SysF.
+From iris.prelude Require Import options.
+From stdpp Require Export base gmap.
+
+
+Module typing.
+(* interesting. since they use autosubst.. 
+forall and exists dont hold types, they hold
+variables of type*)
+Inductive type :=
+  | TUnit : type
+  | TInt : type
+  | TBool : type
+  | TProd : type → type → type
+  | TSum : type → type → type
+  | TArrow : type → type → type
+  | TVar (x : var)
+  | TForall (τ : {bind 1 of type})
+  | TExist (τ : {bind 1 of type}).
+
+Global Instance Ids_type : Ids type. derive. Defined.
+Global Instance Rename_type : Rename type. derive. Defined.
+Global Instance Subst_type : Subst type. derive. Defined.
+Global Instance SubstLemmas_typer : SubstLemmas type. derive. Qed.
+
+
+(* what is this ?*)
+Inductive EqType : type → Prop :=
+  | EqTUnit : EqType TUnit
+  | EqTNat : EqType TInt
+  | EqTBool : EqType TBool.
+
+Reserved Notation "Γ ⊢ₜ e : τ" (at level 74, e, τ at next level).
+
+Import SysF.
+(* note that gamma here is really a type environment *)
+Inductive typed (Γ : list type) : expr → type → Prop :=
+  | Var_typed x τ : Γ !! x = Some τ → Γ ⊢ₜ Var x : τ
+  | Unit_typed : Γ ⊢ₜ Unit : TUnit
+  | Bool_typed b : Γ ⊢ₜ Bool b : TBool
+  | Pair_typed e1 e2 τ1 τ2 :
+     Γ ⊢ₜ e1 : τ1 →
+     Γ ⊢ₜ e2 : τ2 →
+     Γ ⊢ₜ Pair e1 e2 : TProd τ1 τ2
+  | Fst_typed e τ1 τ2 : Γ ⊢ₜ e : TProd τ1 τ2 → Γ ⊢ₜ Fst e : τ1
+  | Snd_typed e τ1 τ2 : Γ ⊢ₜ e : TProd τ1 τ2 → Γ ⊢ₜ Snd e : τ2
+
+  | If_typed e0 e1 e2 τ :
+     Γ ⊢ₜ e0 : TBool → Γ ⊢ₜ e1 : τ → Γ ⊢ₜ e2 : τ → Γ ⊢ₜ If e0 e1 e2 : τ
+  | Lam_typed e τ1 τ2 :
+      τ1 :: Γ ⊢ₜ e : τ2 → Γ ⊢ₜ Lam e : TArrow τ1 τ2
+
+  | App_typed e1 e2 τ1 τ2 :
+     Γ ⊢ₜ e1 : TArrow τ1 τ2 → Γ ⊢ₜ e2 : τ1 → Γ ⊢ₜ App e1 e2 : τ2
+  (* Here are the interesting cases ..
+     autosubst is used again .. which wtf..how?
+  *)
+  | TLam_typed e τ :
+     subst (ren (+1)) <$> Γ ⊢ₜ e : τ → 
+     Γ ⊢ₜ TLam e : TForall τ
+  | TApp_typed e τ τ' : 
+    Γ ⊢ₜ e : TForall τ → 
+    Γ ⊢ₜ TApp e : τ.[τ'/]
+  | Pack_typed e τ τ' :
+     Γ ⊢ₜ e : τ.[τ'/] → 
+     Γ ⊢ₜ Pack e : TExist τ
+  | UnpackIn_typed e1 e2 τ τ' :
+     Γ ⊢ₜ e1 : TExist τ →
+     τ :: (subst (ren (+1)) <$> Γ) ⊢ₜ e2 : τ'.[ren (+1)] →
+     Γ ⊢ₜ UnpackIn e1 e2 : τ'
+where "Γ ⊢ₜ e : τ" := (typed Γ e τ).
+
+
+Fixpoint env_subst (vs : list val) : var → expr :=
+  match vs with
+  | [] => ids
+  | v :: vs' => (of_val v) .: env_subst vs'
+  end.
+
+
+Lemma env_subst_lookup vs x v :
+  vs !! x = Some v → env_subst vs x = of_val v.
+Proof.
+  revert vs; induction x as [|x IH] => vs.
+  - by destruct vs; inversion 1.
+  - destruct vs as [|w vs]; first by inversion 1.
+    apply IH.
+Qed.
+
+
+End typing.
